ainvs: changed definition of `valid_idle` + `idle_tcb_at` ; defined `valid_arch_idle` invariant
* Context :

 We would like to prove that, for ARM_HYP architecture,
 the current vcpu is always the vcpu associated to the current thread.
 See issue https://jira.csiro.au/browse/VER-770
 and PR 291 http://bitbucket.keg.ertos.in.nicta.com.au/projects/SEL4/repos/l4v/pull-requests/291

* Intermediate step : the vcpu of the idle thread is always none

 In this commit, we modify the `valid_idle` invariant so that it includes
  the fact that the vcpu of the idle thread is always None.
 This is needed for PR291 (see Context above).
  `valid_idle` beeing defined with `idle_tcb_at`,
  we changed the definition of `idle_tcb_at`
  so that it can convey information about the architecture.
 And we defined `valid_arch_idle`
  that states that the vcpu of an iarch_tcb is None.

* What changed :

 Even if these changes are only interesting for the
  abstract invariants for arm_hyp architecture
  (that are being extended),
  it implied changes to several generic and architecture-specific
  files of the astract invariants (AInvs) sessions.

Co-authored-by : Corey Lewis <corey.lewis@data61.csiro.au>
Co-authored-by : Santiago Bautista <santiago.bautista@data61.csiro.au>

proof/invariant-abstract/ARM/ArchInvariants_AI.thy
@@ -28,7 +28,13 @@ end_qualify
 section "ARM-specific invariant definitions"
 
 qualify ARM_A (in Arch)
-type_synonym iarch_tcb = unit
+(* ARM has no interest for iarch_tcb (introduced for ARM_HYP) ,
+    and we consider no non-trivial predicates of iarch_tcb,
+    so an unspecified typedecl seems appropriate.
+   In contrast to using a unit type, this avoids
+    over-simplification of idle_tcb_at predicates,
+    which would make it hard to use facts that talk about idle_tcb_at. *)
+typedecl iarch_tcb
 end_qualify
 
 context Arch begin global_naming ARM
@@ -36,7 +42,7 @@ context Arch begin global_naming ARM
 definition
   arch_tcb_to_iarch_tcb :: "arch_tcb \<Rightarrow> iarch_tcb"
 where
-  "arch_tcb_to_iarch_tcb arch_tcb \<equiv> ()"
+  "arch_tcb_to_iarch_tcb arch_tcb \<equiv> undefined"
 
 lemma iarch_tcb_context_set[simp]:
   "arch_tcb_to_iarch_tcb (arch_tcb_context_set p tcb) = arch_tcb_to_iarch_tcb tcb"
@@ -246,6 +252,11 @@ definition
   valid_arch_tcb :: "arch_tcb \<Rightarrow> 'z::state_ext state \<Rightarrow> bool"
 where
   "valid_arch_tcb \<equiv> \<lambda>a. \<top>"
+
+definition
+  valid_arch_idle :: "iarch_tcb \<Rightarrow> bool"
+where
+  "valid_arch_idle \<equiv> \<top>"
 
 primrec
   valid_pte :: "pte \<Rightarrow> 'z::state_ext state \<Rightarrow> bool"
